circular_list.dfy
@@ -1,0 +1,233 @@
+module Circular_List {
+  
+  class Node<T> {
+    var value: T
+      var prev: Node<T>
+      var next: Node<T>
+      ghost var nodes: seq<Node<T> >;
+
+      constructor(x: T) {
+        value := x;
+        prev := this;
+        next := this;
+      }
+  }
+
+  predicate NoDupes<T>(a: seq<T>) {
+    (forall i, j :: 0 <= i < |a| && 0 <= j < |a| && i != j ==> a[i] != a[j])
+  }
+
+  function IndexOf<T(==)>(s: seq<T>, e: T) : int
+    requires e in s;
+    ensures 0 <= IndexOf(s,e) < |s|;
+    ensures s[IndexOf(s,e)] == e;
+  {
+    var i :| 0 <= i < |s| && s[i] == e;
+    i
+  }
+
+  predicate RotationallyEquivalent<T>(a: seq<T>, b: seq<T>) {
+    exists i :: 0 <= i < |b| && a == (b[i..] + b[..i])
+  }
+
+  predicate Valid(node: Node)
+    reads node;
+    reads node.nodes;
+  {
+    var nodes := node.nodes;
+    // We're in the list
+    (node in nodes) &&
+    // Everybody in the list agrees on the list
+    (forall node' :: node' in nodes ==> node'.nodes == nodes) &&
+    // There's no duplicates in the list (technically reduncant but helpful)
+    NoDupes(nodes) &&
+    // next and prevs point right and left in the list, respectively
+    (forall i :: 0 <= i < |nodes|-1 ==> nodes[i].next == nodes[i+1]) &&
+    nodes[|nodes|-1].next == nodes[0] &&
+    (forall i :: 1 <= i < |nodes| ==> nodes[i].prev == nodes[i-1]) &&
+    nodes[0].prev == nodes[|nodes|-1]
+  }
+
+  lemma NextIsValid(node: Node)
+    requires Valid(node);
+    ensures Valid(node.next);
+    ensures node.next in node.nodes;
+    ensures node.next.nodes == node.nodes;
+  {
+    var idx := IndexOf(node.nodes, node);
+    if idx < |node.nodes|-1 {
+      assert node.next == node.nodes[idx + 1];
+    }
+  }
+
+  lemma PrevIsValid(node: Node)
+    requires Valid(node);
+    ensures Valid(node.prev);
+    ensures node.prev in node.nodes;
+    ensures node.prev.nodes == node.nodes;
+  {
+    var idx := IndexOf(node.nodes, node);
+    if idx > 0 {
+      assert node.prev == node.nodes[idx - 1];
+    }
+  }
+
+  lemma PrevNextCancel(n: Node)
+    requires Valid(n);
+    ensures n.next.prev == n;
+  {
+    NextIsValid(n);
+    var idx := IndexOf(n.nodes, n);
+    if idx < |n.nodes|-1 {
+      assert n.next == n.nodes[idx+1];
+    }
+  }
+
+  ghost method BringToFront(a: Node)
+    requires Valid(a);
+    ensures Valid(a);
+    ensures a.nodes == old(a.nodes[IndexOf(a.nodes, a)..]) + old(a.nodes[..IndexOf(a.nodes, a)]);
+    modifies a, a.nodes;
+  {
+    ghost var i := IndexOf(a.nodes, a);
+    ghost var newnodes := a.nodes[i..] + a.nodes[..i];
+    forall a' | a' in a.nodes {
+      a'.nodes := newnodes;
+    }
+  }
+
+  lemma DisjointConcatenation<T(==)>(a: seq<T>, b: seq<T>)
+    requires NoDupes(a);
+    requires NoDupes(b);
+    requires multiset(a) !! multiset(b);
+    ensures NoDupes(a + b);
+  {
+    var c := a + b;
+    if |c| > 1 {
+      assert forall i, j :: i != j && 0 <= i < |a| && |a| <= j < |c| ==>
+        c[i] in multiset(a) && c[j] in multiset(b) && c[i] != c[j]; // Observe
+    }
+  }
+
+  method Splice(a: Node, b: Node)
+    requires Valid(a);
+    requires Valid(b);
+    requires a != b;
+    requires a == a.nodes[0];
+    requires multiset(a.nodes) !! multiset(b.nodes) || a.nodes == b.nodes;
+    requires a.nodes != b.nodes ==> b == b.nodes[0];
+    ensures Valid(a);
+    ensures Valid(b);
+    ensures old(a.nodes) == old(b.nodes) ==>
+      (multiset(a.nodes) !! multiset(b.nodes) &&
+      a.nodes == old(a.nodes[..IndexOf(a.nodes, b)]) &&
+      b.nodes == old(b.nodes[IndexOf(b.nodes, b)..]));
+      ensures multiset(old(a.nodes)) !! multiset(old(b.nodes)) ==>
+        (a.nodes == old(a.nodes) + old(b.nodes) &&
+        a.nodes == b.nodes);
+        modifies a, b, a.nodes, b.nodes;
+  {
+    var a_last := a.prev;
+    var b_last := b.prev;
+
+    assert IndexOf(b.nodes, b) > 0 ==> b_last == b.nodes[IndexOf(b.nodes, b)-1]; // Observe
+
+    a_last.next := b;
+    b_last.next := a;
+    a.prev := b_last;
+    b.prev := a_last;
+
+    if a.nodes != b.nodes {
+      DisjointConcatenation(a.nodes, b.nodes);
+      ghost var newnodes := a.nodes + b.nodes;
+      forall a' | a' in newnodes {
+        a'.nodes := newnodes;
+      }
+    } else {
+      assert |multiset(a.nodes)| > 0; // Observe
+      ghost var newanodes := a.nodes[..IndexOf(a.nodes, b)];
+      ghost var newbnodes := b.nodes[IndexOf(b.nodes, b)..];
+      forall a' | a' in newanodes {
+        a'.nodes := newanodes;
+      }
+      forall b' | b' in newbnodes {
+        b'.nodes := newbnodes;
+      }
+    }
+  }
+
+  predicate Singleton(n: Node)
+    requires Valid(n);
+    reads n, n.nodes;
+  {
+    n.prev == n.next == n
+  }
+
+  lemma SingletonFacts(n: Node)
+    requires Valid(n);
+    requires Singleton(n);
+    ensures n.nodes == [n];
+  {
+    var idx := IndexOf(n.nodes, n);
+    if idx > 0 {
+      assert n.nodes[idx-1] == n;
+    }
+  }
+
+  method InsertAfter(a: Node, b: Node)
+    requires Valid(a);
+    requires Valid(b);
+    requires a != b;
+    requires Singleton(b);
+    ensures Valid(a);
+    ensures Valid(b);
+    ensures a.next == b;
+    ensures a.nodes == old(a.nodes[IndexOf(a.nodes, a)+1..]) + old(a.nodes[..IndexOf(a.nodes, a)+1]) + [b];
+    modifies a, a.nodes, a.next, a.next.nodes, b, b.nodes;
+  {
+    var a' := a.next;
+    SingletonFacts(b);
+    NextIsValid(a);
+    PrevNextCancel(a);
+    BringToFront(a');
+    BringToFront(b);
+    Splice(a', b);
+  }
+
+  lemma NonSingletonFacts(n: Node)
+    requires Valid(n);
+    requires !Singleton(n);
+    ensures Valid(n.next);
+    ensures Valid(n.prev);
+    ensures n.next != n;
+    ensures n.prev != n;
+    ensures |n.nodes| > 1;
+  {
+    NextIsValid(n);
+    PrevIsValid(n);
+    var idx := IndexOf(n.nodes, n);
+    if idx < |n.nodes|-1 {
+      assert n.next == n.nodes[idx+1];
+    }
+    if idx > 0 {
+      assert n.prev == n.nodes[idx-1];
+    }
+  }
+
+  method Remove(n: Node) returns (other: Node)
+    requires Valid(n);
+    requires !Singleton(n);
+    ensures Valid(n);
+    ensures Valid(other);
+    ensures Singleton(n);
+    ensures other.nodes == old(n.nodes[IndexOf(n.nodes,n)+1..]) + old(n.nodes[..IndexOf(n.nodes,n)])
+      modifies n, n.next, n.nodes, n.next.nodes;
+  {
+    BringToFront(n);
+    NonSingletonFacts(n);
+    NextIsValid(n);
+    other := n.next;
+    assert n.nodes[1] == other; // Observe
+    Splice(n, other);
+  }
+}
